Started work on TAPL:
* Defined direct implementations and inductive relations for small-step and large-step evaluation of untyped and typed arithmetic
* Defined direct implementation and inductive relation for typing on typed arithmetic
* Stubbed out several crucial theorems, including:
  * Equivalence of direct implementations and inductive relations where both exist
  * Large-step sematics is the reflexive, transitive closure of the small step sematics
  * Several other theorems from the book

Tapl/Preliminaries.lean
@@ -1,11 +1,29 @@
 /-
 # Mathematical Preleminaries
 -/
-
-/-
-## Sets, Relations, and Functions
--/
-
 import Mathlib.Data.Nat.Basic
 import Mathlib.Data.Finset.Basic
 import Mathlib.Data.Finset.Card
+
+namespace Tapl
+
+  /-
+  ## Sets, Relations, and Functions
+  -/
+
+
+  /-
+  ## Reflexive, Transitive Closure
+  -/
+
+  inductive RTC (R: α → α → Prop): α → α → Prop where
+    | base: ∀ x₁ x₂: α, R x₁ x₂ → RTC R x₁ x₂
+    | refl: ∀ x: α, R x x → RTC R x x
+    | trans: ∀ x₁ x₂ x₃: α, RTC R x₁ x₂ → RTC R x₂ x₃ → RTC R x₁ x₃
+
+  /-
+  ## Deterministic Relations
+  -/
+
+  def deterministic (R: α → α → Prop) (x₁ x₂ x₃: α): R x₁ x₂ → R x₁ x₃ → x₂ = x₃ := sorry
+end Tapl
