Tapl/TyArith.lean
@@ -1,13 +1,15 @@
 /-
-# Untyped Arithmetic
+# Typed Arithmetic
 -/
 
 import «Tapl».«Preliminaries»
 
-import Mathlib.Data.Finset.Basic
-import Mathlib.Data.Finset.Card
+namespace Tapl.TyArith
+  inductive Ty: Type where
+    | bool: Ty
+    | nat: Ty
+  deriving Repr, DecidableEq
 
-namespace Tapl.UntypedArith
   inductive Term: Type where
     | true: Term
     | false: Term
@@ -18,51 +20,51 @@ namespace Tapl.UntypedArith
     | ite: Term → Term → Term → Term
   deriving Repr, DecidableEq
 
-  def Term.consts: Term → Finset Term
-    | .true =>   { .true }
-    | .false => { .false }
-    | .zero => { .zero }
-    | .pred t | .succ t | .isZero t => t.consts
-    | .ite c t f => c.consts ∪ t.consts ∪ f.consts
-
-  def Term.size: Term → Nat
-    | .true | .false | .zero => 1
-    | .pred t | .succ t | .isZero t => 1 + t.size
-    | .ite c t f => 1 + c.size + t.size + f.size
-
-  @[local simp]
-  def Term.depth: Term → Nat
-    | .true | .false | .zero => 1
-    | .pred t | .succ t | .isZero t => 1 + t.depth
-    | .ite c t f => 1 + Nat.max (Nat.max c.depth t.depth) f.depth
-
-  def Term.isNumeric: Term → Bool
-    | .zero => Bool.true
-    | .succ n => n.isNumeric
-    | _ => Bool.false
-
-  def Term.isValue: Term → Bool
-    | .true | .false => Bool.true
-    | t => t.isNumeric
+  def Term.typeOf: Term → Ty
+    | .true => .bool
+    | .false => .bool
+    | .zero => .nat
+    | .pred n =>
+      match n.typeOf with
+        | .nat => .nat
+        | _ => sorry
+    | .succ n =>
+      match n.typeOf with
+        | .nat => .nat
+        | _ => sorry
+    | .isZero n =>
+      match n.typeOf with
+        | .nat => .nat
+        | _ => sorry
+    | .ite c t f =>
+      let tyt := t.typeOf
+      let tyf := f.typeOf
+      match c.typeOf with
+        | .bool =>
+          if tyt == tyf
+          then tyt
+          else sorry
+        | _ => sorry
 
   def Term.eval₁: Term → Term
     | .true => .true
     | .false => .false
     | .zero => .zero
     | .pred .zero => .zero
-    | .pred t => t.eval₁.pred
+    | .pred (.succ n) => n
+    | .pred n => n.eval₁.pred
     | .succ .zero => Term.zero.succ
-    | .succ t => t.eval₁.succ
+    | .succ n => n.eval₁.succ
     | .isZero .zero => .true
     | .isZero (.succ _) => .false
-    | .isZero t => t.eval₁.isZero
+    | .isZero n => n.eval₁.isZero
     | .ite .true t _ => t
     | .ite .false _ f => f
     | .ite c t f => .ite c.eval₁ t f
 
   def Term.eval: Term → Term
     | .true => .true
-    | .false => false
+    | .false => .false
     | .zero => .zero
     | .pred n =>
       match n.eval with
@@ -79,6 +81,15 @@ namespace Tapl.UntypedArith
         | .true => t.eval
         | .false => f.eval
         | _ => sorry
+
+  inductive TypeOf: Term → Ty → Prop where
+    | true: TypeOf Term.true Ty.bool
+    | false: TypeOf Term.false Ty.bool
+    | zero: TypeOf Term.zero Ty.nat
+    | pred (n: Term): TypeOf n Ty.nat → TypeOf n.pred Ty.nat
+    | succ (n: Term): TypeOf n Ty.nat → TypeOf n.succ Ty.nat
+    | isZero (n: Term): TypeOf n Ty.nat → TypeOf n.isZero Ty.nat
+    | ite (c t f: Term) (α: Ty): TypeOf c Ty.bool → TypeOf t α → TypeOf f α → TypeOf (.ite c t f) α
 
   inductive Numeric: Term → Prop where
     | zero: Numeric Term.zero
@@ -110,43 +121,32 @@ namespace Tapl.UntypedArith
     | isZeroZero: ∀ t₁: Term, Eval t₁ .zero → Eval t₁.isZero .true
     | isZeroSucc: ∀ t₁ t₂: Term, Numeric t₂ → Eval t₁ t₂.succ → Eval t₁.isZero .false
 
-  def Term.isNormal: ∀ t₁: Term, ¬ ∃ t₂: Term, Eval t₁ t₂ := sorry
+  theorem typeOf_typeOf: ∀ t: Term, ∀ ty: Ty, TypeOf t ty ↔ t.typeOf = ty := sorry
 
-  theorem eval₁_eval₁ (t₁ t₂: Term): Eval₁ t₁ t₂ ↔ t₁.eval₁ = t₂ := sorry
+  theorem eval₁_eval₁: ∀ t₁ t₂: Term, Eval₁ t₁ t₂ ↔ t₁.eval₁ = t₂ := sorry
 
-  theorem Eval₁.deterministic (t₁ t₂ t₃: Term): Eval₁ t₁ t₂ → Eval₁ t₁ t₃ → t₂ = t₃
-    | .iteTrue t f, h => sorry
-    | .iteFalse t f, h => sorry
-    | .ite c₁ c₂ t f hc, h => sorry
-    | .succ t₁ t₂ t, h => sorry
-    | .predZero, h => sorry
-    | .predSucc t hn, h => sorry
-    | .pred t₁ t₂ ht, h => sorry
-    | .isZeroZero, h => sorry
-    | .isZeroSucc t ht, h => sorry
-    | .isZero t₁ t₂ ht, h => sorry
+  theorem eval_eval: ∀ t₁ t₂: Term, Eval t₁ t₂ ↔ t₁.eval = t₂.eval := sorry
 
-  example (t₁ t₂ t₃: Term): Eval₁ t₁ t₂ → Eval₁ t₁ t₃ → t₂ = t₃ := by
-    intro h₁₂ h₁₃
-    induction h₁₂ with
-      | iteTrue t f => sorry
-      | iteFalse t f => sorry
-      | ite c₁ c₂ t f hc ih => sorry
-      | succ t₁ t₂ t ih => sorry
-      | predZero => sorry
-      | predSucc t hn => sorry
-      | pred t₁ t₂ ht ih => sorry
-      | isZeroZero => sorry
-      | isZeroSucc t ht => sorry
-      | isZero t₁ t₂ ht ih => sorry
+  theorem eval_rtc_eval₁: ∀ t₁ t₂: Term, RTC Eval₁ t₁ t₂ ↔ Eval t₁ t₂ := sorry
 
-  -- theorem Value.normal: ∀ t: Term, Value t → t.isNormal := sorry
+  theorem ty_uniq /-(t: Term) (ty₁ ty₂: Ty)-/ (h₁: TypeOf t ty₁) (h₂: TypeOf t ty₂): ty₁ = ty₂ := by
+    cases h₁ with
+      | true => cases h₂ <;> rfl
+      | false => cases h₂ <;> rfl
+      | zero => cases h₂ <;> rfl
+      | pred n h => cases h₂ <;> rfl
+      | succ n h => cases h₂ <;> rfl
+      | isZero n h => cases h₂ <;> rfl
+      | ite c t f ty h₁ h₂ h₃ =>
+        cases h₂ with
+          | ite c₁ t₂ f₁ ty₁ h₄ h₅ h₆ => sorry
+          | _ => sorry
 
-  theorem eval_eval (t₁ t₂: Term): Eval t₁ t₂ ↔ t₁.eval = t₂ := sorry
+  theorem ty_deriv_uniq: True := sorry
 
-  theorem eval_rtc_eval₁ (t₁ t₂: Term): RTC Eval₁ t₂ t₂ ↔ Eval t₁ t₂ := sorry
+  theorem canonical_forms₁: ∀ t: Term, Value t → TypeOf t Ty.bool → v = Term.true ∨ v = Term.false := sorry
+  theorem canonical_forms₂: ∀ t: Term, Value t → TypeOf t Ty.nat → Numeric v := sorry
 
-  -- theorem normal_unique (t₁ t₂ t₃: Term): t₂.isNormal → t₂.isNormal → Eval t₁ t₂ → Eval t₂ t₃ → t₂ = t₃ := sorry
-
-  -- theorem Eval.termination (t₁: Term): ∃ t₂: Term, t₂.isNormal ∧ Eval t₁ t₂ := sorry
-end Tapl.UntypedArith
+  theorem TypeOf.progress: ∀ t₁: Term, ∀ ty: Ty, TypeOf t₁ ty → Value t₁ ∨ ∃ t₂: Term, Eval₁ t₁ t₂ := sorry
+  theorem TypeOf.preservation: ∀ t₁ t₂: Term, ∀ ty: Ty, TypeOf t₁ ty → Eval₁ t₁ t₂ → TypeOf t₂ ty := sorry
+end Tapl.TyArith
