Tapl.lean
@@ -1,2 +1,3 @@
 import «Tapl».«Preliminaries»
 import «Tapl».«UntypedArith»
+import «Tapl».«TyArith»
